general structure of proof laid out

src/Dmajortodflatmajor.v
@@ -24,7 +24,7 @@ Section PRESERVATION.
 
 Variable prog: Dmajor.program.
 Let ge := Genv.globalenv prog.
-
+Hypothesis no_repet : list_norepet (prog_defs_names prog).
 
 (* Here we have a sufficient condition which we'll prove holds on all stack frames *)
 Definition stack_frame_wf (b : block) (stacksize : Z) (mi : meminj) (m : mem) : Prop :=
@@ -47,6 +47,22 @@ Proof.
   specialize (H1 b' delta). congruence.
 Qed.
 
+Lemma free_stack_frame_inject :
+  forall mi m m' b sz,
+    Mem.inject mi m m' ->
+    stack_frame_wf b sz mi m' ->
+    exists m0,
+      Mem.free m' b 0 sz = Some m0 /\ Mem.inject mi m m0.
+Proof.
+  intros.
+  assert (Mem.mem_inj mi m m') by (inv H; eauto).
+  app free_stack_frame stack_frame_wf. 
+  app Mem.free_right_inject Mem.inject.
+  intros.
+  unfold stack_frame_wf in *. break_and.
+  specialize (H9 b1 delta). congruence.
+Qed.
+
 (* Here we have properties about the memory injection *)
 
 (* This says that our injection maps every old block to something new *)
@@ -65,9 +81,47 @@ Definition env_inj (mi : meminj) (e e' : env) : Prop :=
 
 (* globals aren't moved around *)
 Definition globals_inj_same (mi : meminj) : Prop :=
-  forall i b,
-    Genv.find_symbol ge i = Some b ->
+  forall b f v,
+    (Genv.find_funct_ptr ge b = Some f \/
+    Genv.find_var_info ge b = Some v) ->
     mi b = Some (b,0).
+
+(* yet another useful property for a mapping function *)
+Definition meminj_injective ( mi : meminj) : Prop :=
+  forall b1 b2 b ofs1 ofs2,
+    mi b1 = Some (b, ofs1) ->
+    mi b2 = Some (b, ofs2) ->
+    b1 = b2.
+
+Lemma globals_inj_find_symbol_same :
+  forall i b mi,
+    Genv.find_symbol ge i = Some b ->
+    globals_inj_same mi ->
+    mi b = Some (b,0).
+Proof.
+  intros.
+  app Genv.find_symbol_inversion Genv.find_symbol.
+  unfold prog_defs_names in *.
+  app in_map_iff In. destruct x.
+  simpl in *. subst.
+  unfold globals_inj_same in *.
+  destruct g.
+  app Genv.find_funct_ptr_exists Gfun.
+  unfold ge in *. rewrite H1 in H3. inv H3.
+  eapply H0; eauto.
+  app Genv.find_var_exists Gvar.
+  unfold ge in *. rewrite H1 in H3. inv H3.
+  eapply H0; eauto.
+
+  Unshelve.
+  repeat (econstructor; eauto).
+  repeat (econstructor; eauto).
+Qed.  
+
+Definition same_offsets (mi : meminj) : Prop :=
+  forall b b' delta,
+    mi b = Some (b',delta) ->
+    delta = 0.
 
 (* evaluating expressions translates *)
 Lemma eval_expr_mem_inj :
@@ -78,6 +132,7 @@ Lemma eval_expr_mem_inj :
       total_inj mi m ->
       env_inj mi e e' ->
       globals_inj_same mi ->
+      same_offsets mi ->
       exists v',
         eval_expr ge e' m' sp exp v' /\ Val.inject mi v v'.
 Proof.
@@ -91,6 +146,7 @@ Proof.
     break_match_hyp; try congruence; find_inversion.
     econstructor; eauto.
     break_match; econstructor; eauto.
+    app globals_inj_find_symbol_same Genv.find_symbol.
     ring.
   * edestruct IHeval_expr1; eauto.
     edestruct IHeval_expr2; eauto.
@@ -106,22 +162,53 @@ Proof.
     
     edestruct IHeval_expr; eauto.
     break_and.
-    inv H8.
+    inv H9.
 
     eexists; split.
     econstructor; eauto.
     simpl. 
     erewrite <- H0.
-    f_equal. 
+    f_equal.
     congruence.
 
-    admit. (* whatever *)
+    
+    rewrite Heqo in H12. inv H12.
+    app H5 (mi b).
+    subst delta.
+    rewrite Z.add_0_r.
+    rewrite Int.add_zero. reflexivity.
+    
 
     eauto.
     edestruct IHeval_expr; eauto.
-    break_and. inv H6. congruence.
+    break_and. inv H7. congruence.
 
-Admitted.
+    (* what is this shelf thing? *)
+    Unshelve.
+    eauto.
+Qed.
+
+Lemma eval_exprlist_mem_inj :
+  forall l m e vl,
+    Dmajor.eval_exprlist ge e m l vl ->
+    forall m' mi e' sp,
+      Mem.mem_inj mi m m' ->
+      total_inj mi m ->
+      env_inj mi e e' ->
+      globals_inj_same mi ->
+      same_offsets mi ->
+      exists vl',
+        eval_exprlist ge e' m' sp l vl' /\ Val.inject_list mi vl vl'.
+Proof.
+  induction 1; intros.
+  eexists; split; econstructor; eauto.
+  copy H1.
+  eapply IHeval_exprlist in H1; eauto.
+  break_exists; break_and.
+  eapply eval_expr_mem_inj in H; eauto.
+  break_exists; break_and.
+  eexists; split; econstructor; eauto.
+Qed.  
 
 Inductive match_cont : Dmajor.cont -> Dflatmajor.cont -> Prop :=
 | match_stop :
@@ -140,34 +227,39 @@ Inductive match_cont : Dmajor.cont -> Dflatmajor.cont -> Prop :=
 
 Inductive match_states : Dmajor.state -> Dflatmajor.state -> Prop :=
 | match_state : forall f s k k' b e e' m m' z mi,
-    Mem.mem_inj mi m m' ->
+    Mem.inject mi m m' ->
     stack_frame_wf b (fn_stackspace f) mi m' ->
     match_cont k k' ->
     total_inj mi m ->
     env_inj mi e e' ->
     globals_inj_same mi ->
-    Mem.meminj_no_overlap mi m ->
+    same_offsets mi ->
+    meminj_injective mi ->
     match_states
       (Dmajor.State f s k e m)
       (Dflatmajor.State f s k' (Vptr b Int.zero) e' m' z)
-| match_callstate : forall f args k k' m m' z mi,
-    Mem.mem_inj mi m m' ->
+| match_callstate : forall f args args' k k' m m' z mi,
+    Mem.inject mi m m' ->
     match_cont k k' ->
     total_inj mi m ->
     globals_inj_same mi ->
-    Mem.meminj_no_overlap mi m ->
+    same_offsets mi ->
+    Val.inject_list mi args args' ->
+    meminj_injective mi ->
     match_states
       (Dmajor.Callstate f args k m)
-      (Dflatmajor.Callstate f args k' m' z)
-| match_returnstate : forall v k k' m m' z mi,
-    Mem.mem_inj mi m m' ->
+      (Dflatmajor.Callstate f args' k' m' z)
+| match_returnstate : forall v v' k k' m m' z mi,
+    Mem.inject mi m m' ->
     match_cont k k' ->
     total_inj mi m ->
     globals_inj_same mi ->
-    Mem.meminj_no_overlap mi m ->
+    same_offsets mi ->
+    Val.inject mi v v' ->
+    meminj_injective mi ->
     match_states
       (Dmajor.Returnstate v k m)
-      (Dflatmajor.Returnstate v k' m' z).
+      (Dflatmajor.Returnstate v' k' m' z).
 
 Lemma is_call_cont_transf :
   forall k k',
@@ -186,7 +278,15 @@ Lemma env_inj_set :
       Val.inject mi v x ->
       env_inj mi (PTree.set id v e) (PTree.set id x e').
 Proof.
-Admitted.
+  intros.
+  unfold env_inj in *.
+  intros.
+  destruct (peq id id0) eqn:?. subst.
+  rewrite PTree.gss in *.
+  eexists; split; eauto. congruence.
+  rewrite PTree.gso in * by congruence.
+  eapply H; eauto.
+Qed.
 
 Lemma total_inj_store_mapped :
   forall mi m,
@@ -196,7 +296,130 @@ Lemma total_inj_store_mapped :
       exists b' delta,
         mi b = Some (b',delta).
 Proof.
+  intros.
+  unfold total_inj in *.
+  app Mem.store_valid_access_3 Mem.store.
+  Check Mem.valid_access_load.
+  SearchAbout Mem.valid_access.
+  app Mem.valid_access_implies Mem.valid_access.
+  clear H2.
+  app Mem.valid_access_load Mem.valid_access.
+  edestruct H. eauto.
+  eexists. exists 0. app H (Mem.load c m b ofs).
+  econstructor; eauto.
+Qed.
+
+Lemma stack_frame_wf_store :
+  forall c m b ofs v m',
+    Mem.store c m b ofs v = Some m' ->
+    forall b sz mi,
+      stack_frame_wf b sz mi m ->
+      stack_frame_wf b sz mi m'.
+Proof.
 Admitted.
+
+Lemma total_inj_store :
+  forall c m b ofs v m',
+    Mem.store c m b ofs v = Some m' ->
+    forall mi,
+      total_inj mi m ->
+      total_inj mi m'.
+Proof.
+Admitted.
+
+Lemma no_overlap_store :
+  forall c m b ofs v m',
+    Mem.store c m b ofs v = Some m' ->
+    forall mi,
+      Mem.meminj_no_overlap mi m ->
+      Mem.meminj_no_overlap mi m'.
+Proof.
+Admitted.
+
+
+Lemma symbols_inject_refl :
+  forall mi,
+    globals_inj_same mi ->
+    meminj_injective mi ->
+    symbols_inject mi ge ge.
+Proof.
+  intros.
+  unfold globals_inj_same in *.
+  unfold symbols_inject.
+  split. intros. reflexivity.
+  split. intros.
+  unfold Senv.find_symbol in *.
+  simpl in *.
+  app globals_inj_find_symbol_same Genv.find_symbol.
+  rewrite H1 in H2. inv H2. eauto.
+  split. intros. 
+  unfold Senv.find_symbol in *.
+  simpl in *.
+  app globals_inj_find_symbol_same Genv.find_symbol.
+  intros.
+  unfold Senv.block_is_volatile. simpl.
+  unfold Genv.block_is_volatile.
+  symmetry.
+  break_match.
+  erewrite H in H1; eauto.
+  inv H1. collapse_match. reflexivity.
+  
+  break_match; auto.
+  assert (mi b2 = Some (b2, 0)) by (eapply H; eauto).
+  unfold meminj_injective in *.
+  erewrite (H0 b1) in Heqo by eauto; congruence.
+  Unshelve.
+  repeat (econstructor; eauto).
+  repeat (econstructor; eauto).
+Qed.  
+
+Lemma match_call_cont :
+  forall k k',
+    match_cont k k' ->
+    match_cont (Dmajor.call_cont k) (call_cont k').
+Proof.
+  induction 1; intros; simpl; eauto; try solve [econstructor; eauto].
+Qed.
+
+(* TODO: this lemma is duplicated from Emajortodmajor, make unified memory library *)
+Lemma alloc_store :
+  forall m lo hi m' b,
+    Mem.alloc m lo hi = (m',b) ->
+    forall v c,
+      hi - lo > size_chunk c ->
+      (align_chunk c | lo) ->
+      { m'' : mem | Mem.store c m' b lo v = Some m''}.
+Proof.
+  intros.
+  app Mem.valid_access_alloc_same Mem.alloc; try omega.
+  app Mem.valid_access_implies Mem.valid_access.
+  2: instantiate (1 := Writable); econstructor; eauto.
+  eapply Mem.valid_access_store; eauto.
+Qed.
+
+Lemma alloc_store_inject :
+  forall m lo hi m' b c m'' v,
+    Mem.alloc m lo hi = (m',b) ->
+    Mem.store c m' b lo v = Some m'' ->
+    forall mi m0 v',
+      Mem.inject mi m m0 ->
+      Val.inject mi v v' ->
+      total_inj mi m ->
+      globals_inj_same mi ->
+      same_offsets mi ->
+      meminj_injective mi ->
+      exists m0' m0'' b',
+      let mi' := (fun x => if peq x b then Some (b',0) else mi x) in
+        Mem.alloc m0 lo hi = (m0',b') /\
+        Mem.store c m0' b' lo v' = Some m0'' /\
+        Mem.inject mi' m'' m0'' /\
+        total_inj mi' m'' /\
+        globals_inj_same mi' /\
+        same_offsets mi' /\
+        meminj_injective mi'.
+Proof.
+Admitted.
+
 
 Lemma single_step_correct:
   forall S1 t S2, Dmajor.step ge S1 t S2 ->
@@ -207,26 +430,142 @@ Proof.
   
   inv H0; inv H;
   try solve [inv H3;
-             eexists; split; try eapply plus_one; econstructor; eauto].
-  * app free_stack_frame stack_frame_wf; eauto.
+             eexists; split; try eapply plus_one; econstructor; eauto];
+  do 3 (try match goal with
+        | [ H : Dmajor.eval_expr _ _ _ _ _ |- _ ] => eapply eval_expr_mem_inj in H; repeat break_exists; repeat break_and; try eassumption
+        | [ H : Dmajor.eval_exprlist _ _ _ _ _ |- _ ] => eapply eval_exprlist_mem_inj in H; repeat break_exists; repeat break_and; try eassumption
+            end);
+  match goal with
+  | [ H : Mem.inject _ _ _ |- Mem.mem_inj _ _ _ ] => solve [inversion H; eassumption]
+  | [ |- _ ] => idtac
+  end;
+  match goal with
+  | [ H : Mem.inject ?X ?Y ?Z |- _ ] =>
+    assert (Mem.mem_inj X Y Z) by (inversion H; auto)
+  end.
+
+  * app free_stack_frame_inject stack_frame_wf; eauto.
     eexists; split; try eapply plus_one; econstructor; eauto.
     eapply is_call_cont_transf; eauto.
-  * app eval_expr_mem_inj Dmajor.eval_expr.
-    eexists; split; try eapply plus_one; econstructor; eauto.
+  * eexists; split; try eapply plus_one; econstructor; eauto.
     eapply env_inj_set; eauto.
-  * app eval_expr_mem_inj (Dmajor.eval_expr ge e m addr vaddr).
-    app eval_expr_mem_inj (Dmajor.eval_expr ge e m a v).
-    destruct vaddr; simpl in *; try congruence.
+  * destruct vaddr; simpl in *; try congruence.
     app total_inj_store_mapped total_inj.
-    app Mem.store_mapped_inj Mem.mem_inj.
-    inv H10.    
+    app Mem.store_mapped_inject Mem.inject; try solve [invp Mem.inject; eauto].
+    invp (Val.inject mi (Vptr b0 i)).
+    eexists; split; try eapply plus_one; econstructor;
+      try solve [
+            eapply stack_frame_wf_store; eauto];
+      eauto.
+    simpl. 
+    find_rewrite.
+    match goal with
+    | [ H : Some _ = Some _ |- _ ] => inv H
+    end.
+    match goal with
+    | [ H : same_offsets _, H2 : mi _ = Some _ |- _ ] =>
+      eapply H in H2; subst
+    end.
+    rewrite Int.add_zero. rewrite Z.add_0_r in *. eauto.
+    eapply total_inj_store; eauto.
+  * eexists; split; try eapply plus_one; econstructor; eauto.
+    destruct vfp; simpl in *; try congruence.
+    unfold Genv.find_funct in *.
+    break_match_hyp; try congruence. subst i.
+    invp (Val.inject mi (Vptr b0 Int.zero)).
+    match goal with
+    | [ H : globals_inj_same _, H2 : mi _ = Some _ |- _ ] =>
+      erewrite H in H2; eauto
+    end.
+    match goal with
+    | [ H : Some _ = Some _ |- _ ] => inv H
+    end.
+    rewrite Int.add_zero. break_match; try congruence.
+    econstructor; eauto.
+  * invp external_call.
+    invp Val.inject.
+    app alloc_store_inject Mem.store.
+    match goal with
+    | [ H : let _ := _ in _ |- _ ] => destruct H
+    end.
+    repeat break_and.
+    eexists; split; try eapply plus_one; econstructor;
+      match goal with
+      | [ |- external_call _ _ _ _ _ _ _ ] => econstructor; eauto
+      | [ |- _ ] => idtac
+      end;
+      eauto.
+
+    (* stack frame: not exactly sure where to go here *)
+    (* need to stick invariant in match_cont about all things being stack_frame_wf *)
+    admit.
+
+    (* just env_inj proof here *)
+    {
+      unfold env_inj. intros.
+
+      destruct (peq id id0) eqn:?.
+      subst. rewrite PTree.gss in *.
+      eexists; split; eauto.
+      match goal with
+      | [ H : Some _ = Some _ |- _ ] => inv H
+      end.
+      econstructor; eauto. break_if; try congruence.
+      reflexivity.
+      ring.
+
+      rewrite PTree.gso in * by congruence.
+      unfold env_inj in *.
+      app H5 (e ! id0).
+      eexists; split; eauto.
+      inv H24; econstructor; eauto.
+      find_rewrite.
+      break_match; try congruence.
+      (* This case is weird, idk *)
+      admit.
+    } 
+
+  * eexists; split; try eapply plus_one; econstructor; eauto.
+    econstructor; eauto.
+  * eexists; split; try eapply plus_one; econstructor; eauto.
+    econstructor; eauto.
+  * eexists; split; try eapply plus_one; econstructor; eauto.
+    inv H17; inv H10; econstructor; eauto.
+  * app free_stack_frame_inject stack_frame_wf.
     eexists; split; try eapply plus_one; econstructor; eauto.
-    simpl. rewrite <- H1.
-    f_equal; try congruence.
-    admit. (* grumble ints *)
+    eapply match_call_cont; eauto.
+  * app free_stack_frame_inject stack_frame_wf.
+    eexists; split; try eapply plus_one; econstructor; eauto; try eapply match_call_cont; eauto.
+  * (* This is an interesting one *)
+    (* we have to allocate memory *)
+    (* but we don't have to stick it in the injection *)
+    
+    admit.
+  * inv H2.
+    eexists; split; try eapply plus_one; try econstructor; eauto.
+    (* match_cont needs Kcall to contain a Vptr for sp *)
+    admit.
 
-
-  
+    
+Unshelve.
+repeat (econstructor; eauto).
+repeat (econstructor; eauto).
+repeat (econstructor; eauto).
+repeat (econstructor; eauto).
+repeat (econstructor; eauto).
+repeat (econstructor; eauto).
+repeat (econstructor; eauto).
+repeat (econstructor; eauto).
+repeat (econstructor; eauto).
+repeat (econstructor; eauto).
+repeat (econstructor; eauto).
+repeat (econstructor; eauto).
+repeat (econstructor; eauto).
+repeat (econstructor; eauto).
+repeat (econstructor; eauto).
+repeat (econstructor; eauto).
+repeat (econstructor; eauto).
+    
 Admitted.
 
 End PRESERVATION.
